More prefascism.

forcing_uip/cwf.v
@@ -2,11 +2,12 @@ Set Primitive Projections.
 Set Universe Polymorphism.
 Set Polymorphic Inductive Cumulativity.
 
+Inductive True : SProp := I.
+Inductive False : SProp :=.
+Inductive and (A : SProp) (B : SProp) : SProp := conj : A -> B -> and A B.
+
 Axiom F : False.
 Ltac admit := case F.
-
-Inductive True : SProp := I.
-Inductive and (A : SProp) (B : SProp) : SProp := conj : A -> B -> and A B.
 
 Set Definitional UIP.
 
@@ -68,6 +69,13 @@ Coercion sub_fun : Sub >-> Funclass.
 
 Arguments sub_fun {_ _}.
 Arguments sub_rel {_ _}.
+
+(*
+Definition Cmp {Γ Δ Ξ : Ctx} (σ : Sub Γ Δ) (ρ : Sub Δ Ξ) : Sub Γ Ξ.
+Proof.
+unshelve econstructor.
++ refine (fun p γ γε => ρ _ _ (fun q α => σ.(sub_rel) _ (α · γ) (α · γε))).
+*)
 
 Record Typ (Γ : Ctx) := {
   typ_typ : forall p
@@ -135,76 +143,121 @@ Arguments ext_typ_ctx {_ _ _}.
 Arguments ext_typ_rel {_ _ _}.
 Arguments ext_typ_ext {_ _ _}.
 
-Record Ext_rel (Γ : Ctx) (A : Typ Γ) (p : ℙ)
-  (γ : forall q : ℙ, q ≤ p -> Ext_typ Γ A q) : SProp := {
-
-  ext_rel_ctx :
-    forall q (α : q ≤ p),
-      eqn (γ q α).(ext_typ_ctx) (fun r (β : r ≤ q) => (γ r (β ∘ α)).(ext_typ_ctx) r !);
-
-  ext_rel_ext :
-
-    forall q (α : q ≤ p),
-    @typ_rel _ A q
-      (fun r (β : r ≤ q) => (γ r (β ∘ α)).(ext_typ_ctx) r !)
-      (rew
-        (fun γ₀ => forall r (β : r ≤ q), ctx_rel Γ (β · γ₀))
-        (ext_rel_ctx q α)
-        ((γ q α).(ext_typ_rel))
-      )
-      (fun r (β : r ≤ q) =>
-        eqn_rect
-          (fun
-            (γ₀ : forall q : ℙ, q ≤ r -> Γ q)
-            (e₀ : eqn (ext_typ_ctx (γ r (β ∘ α))) γ₀) =>
-              A r γ₀ (rew (fun γ₀ => forall (s : ℙ) (ζ : s ≤ r), ctx_rel Γ (ζ · γ₀)) e₀ _)
-        )
-        (γ r (β ∘ α)).(ext_typ_ext)
-        (ext_rel_ctx r (β ∘ α))
-      )
-
-}.
-
-Arguments ext_rel_ctx {_ _ _ _}.
-Arguments ext_rel_ext {_ _ _ _}.
-
-Definition Θ {Γ : Ctx} (p : ℙ)
+Definition Θ {Γ : Ctx} {p : ℙ}
   (γ : forall (q : ℙ) (α : q ≤ p) r (β : r ≤ q), Γ r)
   (γε : forall (q : ℙ) (α : q ≤ p) r (β : r ≤ q), ctx_rel Γ (β · (γ q α)))
   (γe : forall q (α : q ≤ p), eqn (γ q α) (fun r (β : r ≤ q) => (γ r (β ∘ α)) r !)) :
   forall (q : ℙ) (α : q ≤ p),
     ctx_rel Γ (fun  (r : ℙ) (β : r ≤ q) => γ r (β ∘ α) r !) :=
   rew (fun γ₀ => forall q (α : q ≤ p), ctx_rel Γ (α · γ₀)) (γe p !) (γε p !).
-(*
-Definition FreeE {Γ : Ctx} (p : ℙ)
+
+Definition letΘ {Γ : Ctx} {A : Typ Γ} {p : ℙ}
   (γ : forall (q : ℙ) (α : q ≤ p) r (β : r ≤ q), Γ r)
   (γε : forall (q : ℙ) (α : q ≤ p) r (β : r ≤ q), ctx_rel Γ (β · (γ q α)))
   (γe : forall q (α : q ≤ p), eqn (γ q α) (fun r (β : r ≤ q) => (γ r (β ∘ α)) r !))
-  (A : forall
-    (γ : forall q : ℙ, q ≤ p -> Γ q)
-    (γε : forall (q : ℙ) (α : q ≤ p), ctx_rel Γ (α · γ)), Type)
-  (x : forall q (α : q ≤ p), A (γ p !) (γε p !))
+  (x : forall q (α : q ≤ p), A q (γ q α) (γε q α)) :
+  (forall (q : ℙ) (α : q ≤ p), A q (fun r β => γ r (β ∘ α) r !) (α · Θ _ γε γe)).
+Proof.
+refine (fun q (α : q ≤ p) =>
+  eqn_rect
+    (fun
+      (γ₀ : forall r : ℙ, r ≤ q -> Γ r)
+      (e₀ : eqn (γ q α) γ₀) =>
+        A q γ₀ (rew (fun γ₀ => forall (r : ℙ) (β : r ≤ q), ctx_rel Γ (β · γ₀)) e₀ (γε q α))
+  )
+  (x q α)
+  (γe q α)
+).
+Defined.
+
+Definition eqn_sym {A} {x y : A} (e : eqn x y) : eqn y x.
+Proof.
+destruct e; reflexivity.
+Qed.
+
+(*
+Lemma letΘ_rect {Γ : Ctx} {A : Typ Γ} {p : ℙ}
+  (P :
+    forall
+      (γ : forall (q : ℙ) (α : q ≤ p), Γ q)
+      (γε : forall (q : ℙ) (α : q ≤ p), ctx_rel Γ (α · γ))
+      (x : forall (q : ℙ) (α : q ≤ p), A q (α · γ) (α · γε)),
+      Type
+  )
+  (γ : forall (q : ℙ) (α : q ≤ p) r (β : r ≤ q), Γ r)
+  (γε : forall (q : ℙ) (α : q ≤ p) r (β : r ≤ q), ctx_rel Γ (β · (γ q α)))
+  (γe : forall q (α : q ≤ p), eqn (γ q α) (fun r (β : r ≤ q) => (γ r (β ∘ α)) r !))
+  (x : forall q (α : q ≤ p), A q (γ q α) (γε q α))
+(*   (u : P γ γε x) *)
   :
-  True.
+  P (fun q (α : q ≤ p) => γ q α q !) (Θ γ γε γe) (@letΘ Γ A p γ γε γe x).
 Proof.
 
-pose (fun q (α : q ≤ p) r (β : r ≤ q) =>
-        eqn_rect
-          (fun
-            (γ₀ : forall q : ℙ, q ≤ r -> Γ q)
-            (e₀ : eqn ((γ r (β ∘ α))) γ₀) =>
-              A r γ₀ (rew (fun γ₀ => forall (s : ℙ) (ζ : s ≤ r), ctx_rel Γ (ζ · γ₀)) e₀ _)
-        )
-        (γ r (β ∘ α)).(ext_typ_ext)
-        (ext_rel_ctx r (β ∘ α))
-      ).
+unshelve refine (let F :=
+
+  (fun
+    (γ₀ : forall q (α : q ≤ p), Γ q)
+    (e₀ : eqn (γ p !) γ₀) =>
+    P γ₀
+      (rew (fun γ₀ => forall q (α : q ≤ p), ctx_rel Γ (α · γ₀)) e₀ (γε p !))
+      (fun q α => eqn_rect
+        (fun γ₁ e₁ => A q (α · γ₁) (α · (rew (fun γ₂ => forall r β, ctx_rel Γ (β · γ₂)) e₁ (γε p !))))
+        _
+        e₀)
+  )
+
+in _
+
+
+).
+
+simpl.
+
+unshelve refine (
+
+eqn_rect (fun γ₁ (e₁ : eqn (fun q (α : q ≤ p) => γ q α q !) γ₁) =>
+  forall e,
+  A q (α · γ₁)
+    (e : forall (r : ℙ) (β : r ≤ q), ctx_rel Γ ((β ∘ α) · γ₁))
+) _ (eqn_sym (γe p !)) _
+
+).
+
+simpl.
+Admitted.
 *)
+
+
+Record Ext_rel (Γ : Ctx) (A : Typ Γ) (p : ℙ)
+  (γ : forall q (β : q ≤ p) r (β : r ≤ q), Γ r)
+  (γε : forall q (α : q ≤ p) r (β : r ≤ q), ctx_rel Γ (β · (γ q α)))
+  (x : forall q (α : q ≤ p), A q (γ q α) (γε q α)) : SProp := {
+
+  ext_rel_ctx :
+    forall q (α : q ≤ p),
+      eqn (γ q α) (fun r (β : r ≤ q) => (γ r (β ∘ α)) r !);
+
+  ext_rel_ext :
+    forall q (α : q ≤ p),
+    @typ_rel _ A q
+      (fun r (β : r ≤ q) => (γ r (β ∘ α)) r !)
+      (Θ _ (fun r β => (γε r (β ∘ α))) (α · ext_rel_ctx))
+      (letΘ _ _ (α · ext_rel_ctx) (fun r β => (x r (β ∘ α))))
+}.
+
+Arguments ext_rel_ctx {_ _ _ _ _ _}.
+Arguments ext_rel_ext {_ _ _ _ _ _}.
 
 Definition Ext (Γ : Ctx) (A : Typ Γ) : Ctx.
 Proof.
 unshelve econstructor.
 + refine (Ext_typ Γ A).
-+ refine (Ext_rel Γ A).
++ refine (fun p γ =>
+  Ext_rel Γ A p
+    (fun q α => (γ q α).(ext_typ_ctx))
+    (fun q α => (γ q α).(ext_typ_rel))
+    (fun q α => (γ q α).(ext_typ_ext))
+).
 Defined.
 
 Definition Cns (Γ : Ctx) (A : Typ Γ) (t : Trm Γ A) : Sub Γ (Ext Γ A).
@@ -226,8 +279,8 @@ unshelve econstructor; simpl.
 + refine (fun p γ γε => (γ p !).(ext_typ_ctx) p !).
 + simpl.
   intros p γ γε.
-  refine (rew (fun γ₀ => ctx_rel Γ γ₀) ((γε p !).(ext_rel_ctx) p !) _).
-  refine ((γ p !).(ext_typ_rel) p !).
+  refine (Θ _ _ ((γε p !).(ext_rel_ctx)) p !).
+  refine (fun q α => (γ q α).(ext_typ_rel)).
 Defined.
 
 Definition Lft {Γ Δ : Ctx} (σ : Sub Γ Δ) (A : Typ Δ) :
@@ -236,14 +289,8 @@ Proof.
 unshelve econstructor.
 + unshelve refine (fun p γ γε => Build_Ext_typ _ _ _ _ _ _); simpl in *.
   - unshelve refine (fun q α => σ q (fun r (β : r ≤ q) => (γ r (β ∘ α)).(ext_typ_ctx) r !) _).
+    refine (Θ _ (fun r β => (γ r (β ∘ α)).(ext_typ_rel)) (fun r β => (γε r (β ∘ α)).(ext_rel_ctx) r !)).
 
-(*     refine (Θ _ _ (fun r β => (γ r (β ∘ α)).(ext_typ_rel)) (fun r β => (γε r (β ∘ α)).(ext_rel_ctx) r !)). *)
-    refine ((rew
-            (fun γ₀ => forall r (β : r ≤ q), ctx_rel Γ (β · γ₀))
-            (ext_rel_ctx (γε q α) q !)
-            ((γ q α).(ext_typ_rel))
-          )
-    ).
   - refine (fun q α => σ.(sub_rel) q
       (fun r (β : r ≤ q) => (γ r (β ∘ α)).(ext_typ_ctx) r !)
       (rew (fun γ₀ => forall r (β : r ≤ q), ctx_rel Γ (β · γ₀)) ((γε q α).(ext_rel_ctx) q !) (γ q α).(ext_typ_rel))
@@ -273,16 +320,11 @@ Definition Var {Γ : Ctx} {A : Typ Γ} : Trm (Ext Γ A) (Typ_subs (Wkn Γ A) A).
 Proof.
 unshelve econstructor; simpl.
 + refine (fun p γ γε => _).
-  refine (
-    eqn_rect
-      (fun γ₀ (e₀ : eqn (ext_typ_ctx (γ p !)) γ₀) =>
-        A p γ₀ (rew (fun γ₀ => forall q (α : q ≤ p), ctx_rel Γ (α · γ₀)) e₀ (γ p !).(ext_typ_rel))
-      )
-      (γ p !).(ext_typ_ext)
-      ((γε p !).(ext_rel_ctx) p !)).
+  refine (letΘ _ (fun q α => (γ q α).(ext_typ_rel)) (fun q α => (γε q α).(ext_rel_ctx) q !) _ p !).
+  refine (fun q α => (γ q α).(ext_typ_ext)).
 + simpl.
   refine (fun p γ γε => _).
-  refine (@ext_rel_ext _ _ _ _ (γε p !) p !).
+  refine (@ext_rel_ext _ _ _ _ _ _ (γε p !) p !).
 Defined.
 
 Definition Prd {Γ : Ctx} (A : Typ Γ) (B : Typ (Ext Γ A)) : Typ Γ.
@@ -350,6 +392,8 @@ Proof.
 reflexivity.
 Qed.
 
+(** Universes *)
+
 Record TYPE@{i} (p : ℙ) : Type@{i+1} := {
   elt : forall q (α : q ≤ p), Type@{i};
   rel : (forall q (α : q ≤ p), elt q α) -> SProp;
@@ -374,3 +418,288 @@ unshelve econstructor.
   refine ((A.(trm_elt) p γ γε).(rel) _).
   refine (eqn_rect (fun A₀ _ => forall q (α : q ≤ p), A₀ q α) x (A.(trm_rel) p γ γε)).
 Defined.
+
+Definition Rfl {Γ : Ctx} (A : Typ Γ) : Trm Γ Unv.
+Proof.
+unshelve econstructor; simpl.
++ refine (fun p γ γε => _).
+  unshelve econstructor.
+  - refine (fun q α => A.(typ_typ _) q (α · γ) (α · γε)).
+  - refine (A.(typ_rel)).
++ reflexivity.
+Defined.
+
+Lemma Rfl_Elt : forall (Γ : Ctx) (A : Typ Γ), Elt (Rfl A) = A.
+Proof.
+reflexivity.
+Qed.
+
+(** Natural numbers *)
+
+Inductive Nat₀ (p : ℙ) :=
+| O₀ : Nat₀ p
+| S₀ : forall (n : forall q (α : q ≤ p), Nat₀ q), Nat₀ p.
+
+Inductive Natε {p : ℙ} : (forall q (α : q ≤ p), Nat₀ q) -> SProp :=
+| Oε : Natε (fun q _ => O₀ q)
+| Sε : forall (n : forall q (α : q ≤ p), Nat₀ q) (nε : forall q (α : q ≤ p), Natε (α · n)),
+      Natε (fun q α => S₀ q (α · n)).
+
+Definition Nat {Γ : Ctx} : Typ Γ.
+Proof.
+unshelve econstructor.
++ refine (fun p γ γε => _).
+  exact (Nat₀ p).
++ refine (fun p γ γε n => _).
+  exact (Natε n).
+Defined.
+
+Definition O {Γ : Ctx} : Trm Γ Nat.
+Proof.
+unshelve econstructor.
++ refine (fun p γ γε => O₀ p).
++ simpl; refine (fun p γ γε => Oε).
+Defined.
+
+Definition S {Γ : Ctx} : Trm Γ (Prd Nat Nat).
+Proof.
+unshelve econstructor.
++ simpl; refine (fun p γ γε n nε => S₀ p n).
++ simpl; refine (fun p γ γε q α n nε => Sε n nε).
+Defined.
+
+Definition Nat_O_inv (p : ℙ)
+    (n : forall q : ℙ, q ≤ p -> Nat₀ q)
+    (nε : forall (q : ℙ) (α : q ≤ p), Natε (α · n))
+    (e : eqn (O₀ p) (n p !)) :
+    eqn (fun q _ => O₀ q) n.
+Proof.
+specialize (nε p !).
+change (Natε n) in nε.
+destruct nε.
++ reflexivity.
++ let t := match type of e with eqn _ ?t => t end in
+  elimtype False;
+  change (match t with O₀ _ => True | S₀ _ n => False end).
+  destruct e; constructor.
+Qed.
+
+Definition Nat_S_inv (p : ℙ)
+    (n : forall q : ℙ, q ≤ p -> Nat₀ q)
+    (nε : forall (q : ℙ) (α : q ≤ p), Natε (α · n))
+    (m : forall q : ℙ, q ≤ p -> Nat₀ q)
+    (e : eqn (S₀ p m) (n p !)) :
+    eqn (fun q α => S₀ q (α · m)) n.
+Proof.
+specialize (nε p !).
+change (Natε n) in nε.
+destruct nε.
++ let t := match type of e with eqn _ ?t => t end in
+  elimtype False;
+  change (match t with S₀ _ _ => True | O₀ _ => False end).
+  destruct e; constructor.
++ refine (
+    match e in eqn _ z return
+      match z return SProp with
+      | O₀ _ => True
+      | S₀ _ n₀ => eqn (fun q α => S₀ q (α · m)) (fun q α => S₀ q (α · n₀))
+      end
+    with refl _ _ => refl _ _ end
+  ).
+Qed.
+
+Definition Build_trm_aux {Γ : Ctx} (A : Typ Γ)
+  (x : forall (p : ℙ)
+    (γ : forall q (α : q ≤ p), Γ q)
+    (γε : forall q (α : q ≤ p), (ctx_rel Γ) (α · γ)),
+    exist
+    (forall q (α : q ≤ p), A q (α · γ) (α · γε))
+    (fun x => @typ_rel _ A p γ γε x))
+  (xε : forall p
+    (γ : forall q (α : q ≤ p), Γ q)
+    (γε : forall q (α : q ≤ p), (ctx_rel Γ) (α · γ)),
+    eqn ((x p γ γε).(val)) (fun q (α : q ≤ p) => (x q (α · γ) (α · γε)).(val) q !)) :
+  Trm Γ A.
+Proof.
+unshelve econstructor.
++ intros p γ γε.
+  refine ((x p γ γε).(val) p !).
++ simpl; intros p γ γε.
+  refine (rew (fun x₀ => typ_rel A x₀) (xε p γ γε) _).
+  refine ((x p γ γε).(spc)).
+Defined.
+
+(*
+Definition foo
+
+{Γ : Ctx} (A : Typ Γ) (B : Typ (Ext Γ A)) p
+
+    (γ : forall q (α : q ≤ p), Γ q)
+    (γε : forall q (α : q ≤ p), (ctx_rel Γ) (α · γ))
+    (x : forall q (α : q ≤ p), A q (α · γ) (α · γε))
+    (xε : forall q (α : q ≤ p), @typ_rel _ A _ (α · γ) (α · γε) (α · x)) :
+    Type
+.
+unshelve refine (
+
+    exist
+    (forall q (α : q ≤ p), B q
+      (fun r β => Build_Ext_typ Γ A r
+        ((β ∘ α) · γ) ((β ∘ α) · γε) (x r (β ∘ α)))
+      (fun r β => Build_Ext_rel Γ A r _ _ _ _ _))
+    (fun x => (* @typ_rel _ B _ _ _ _ *) _)
+
+).
+
+simpl.
+intros; reflexivity.
+simpl.
+Show Proof.
+
+
+Definition Build_lam_aux {Γ : Ctx} (A : Typ Γ) (B : Typ (Ext Γ A))
+  (f : forall (p : ℙ)
+    (γ : forall q (α : q ≤ p), Γ q)
+    (γε : forall q (α : q ≤ p), (ctx_rel Γ) (α · γ))
+    (x : forall q (α : q ≤ p), A q (α · γ) (α · γε))
+    (xε : forall q (α : q ≤ p), @typ_rel _ A _ (α · γ) (α · γε) (α · x)),
+    exist
+    (forall q (α : q ≤ p), A q (α · γ) (α · γε))
+    (fun x => @typ_rel _ A p γ γε x))
+(*
+  (xε : forall p
+    (γ : forall q (α : q ≤ p), Γ q)
+    (γε : forall q (α : q ≤ p), (ctx_rel Γ) (α · γ)),
+    eqn ((x p γ γε).(val)) (fun q (α : q ≤ p) => (x q (α · γ) (α · γε)).(val) q !)) :
+*)
+  :
+  Trm (Ext Γ A) B.
+Proof.
+unshelve econstructor.
++ intros p γ γε.
+  refine ((x p γ γε).(val) p !).
++ simpl; intros p γ γε.
+  refine (rew (fun x₀ => typ_rel A x₀) (xε p γ γε) _).
+  refine ((x p γ γε).(spc)).
+Defined.
+*)
+
+Definition Ext_elim₀  {Γ : Ctx} (A : Typ Γ) (p : ℙ)
+  (P : forall
+    (γ : forall q : ℙ, q ≤ p -> Ext Γ A q)
+    (γε : forall (q : ℙ) (α : q ≤ p), ctx_rel (Ext Γ A) (α · γ)), Type)
+  (u : forall
+    (γ : forall q (α : q ≤ p) r (β : r ≤ q), Γ r)
+    (γε : forall q (α : q ≤ p) r (β : r ≤ q), ctx_rel Γ (β · (γ q α)))
+    (x : forall q (α : q ≤ p), A q (γ q α) (γε q α))
+    (γe : forall q (α : q ≤ p),
+                 eqn (γ q α) (fun (r : ℙ) (β : r ≤ q) => γ r (β ∘ α) r !))
+    (xε : forall q (α : q ≤ p), @typ_rel Γ A q (fun (r : ℙ) (β : r ≤ q) => γ r (β ∘ α) r !) (α · Θ γ γε γe) (letΘ (α · γ) (α · γε) (α · γe) (α · x))),
+    P (fun q α => Build_Ext_typ Γ A q (γ q α) (γε q α) (x q α))
+    (fun q α => Build_Ext_rel Γ A q (α · γ) (α · γε) (α · x) (α · γe) (α · xε))
+
+  )
+  (γ : forall q (α : q ≤ p), Ext Γ A q)
+  (γε : forall q (α : q ≤ p), ctx_rel (Ext Γ A) (α · γ)) :
+  P γ γε.
+Proof.
+refine (u
+  (fun q α r β => (γ q α).(ext_typ_ctx) r β)
+  (fun q α r β => (γ q α).(ext_typ_rel) r β)
+  (fun q α => (γ q α).(ext_typ_ext))
+  (fun q α => (γε q α).(ext_rel_ctx) q !)
+  (fun q α => (γε q α).(ext_rel_ext) q !)
+).
+Defined.
+
+Definition Nat_rect {Γ : Ctx}
+  (P : Trm Γ (Prd Nat Unv))
+  (pO : Trm Γ (Elt (App P O)))
+  (pS : Trm Γ
+    (Prd Nat
+    (Prd (Elt (@App _ Nat Unv (Trm_subs (Wkn _ _) P) (@Var _ Nat)))
+      (Elt (@App _ Nat Unv ((Trm_subs (Wkn (Ext Γ Nat) _)
+      (Trm_subs (Wkn Γ Nat) P))) (App S (Trm_subs (Wkn (Ext Γ Nat) _) Var)))))))
+  :
+  Trm Γ (Prd Nat (Elt ((@App _ Nat Unv (Trm_subs (Wkn _ _) P)) (@Var _ Nat)))).
+Proof.
+unshelve refine (Lam _ _).
+unshelve refine (Build_trm_aux _ (fun p => _) _).
++ refine (@Ext_elim₀ Γ Nat p _ _); simpl.
+  intros γ γε n γe nε.
+  generalize (refl _ (n p !)).
+  generalize (n p !) at 1 as n₀.
+  induction n₀ as [|p n₀ IHn₀]; intros e₀.
+  - simpl; unshelve econstructor.
+    refine (fun q α => _).
+    change (
+      elt
+        (trm_elt P q (fun (q0 : ℙ) (α0 : q0 ≤ q) => γ q0 (α0 ∘ α) q0 !)
+           (Θ (α · γ) (α · γε) (α · γe))
+           (@letΘ Γ Nat _ (α · γ) (α · γε) (α · γe) (α · n)) (α · nε)) q !
+    ).
+    assert (nε' : Na
+
+pose (Nat_O_inv _ (@letΘ Γ Nat _ γ γε γe n) nε).
+
+(letΘ _
+       _
+       _
+       (fun r β => (γ r β).(ext_typ_ext)))
+
+) (fun r β => (γε r β).(ext_rel_ext) r !) e₀).
+pose (u := pO.(trm_elt) q (fun r β => ext_typ_ctx (γ r (β ∘ α)) r !)).
+simpl in u.
+
+
+    { refine (fun q α => _).
+
+(*       pose (e₁ := (γε p !).(ext_rel_ctx) p !). *)
+
+      refine (
+
+        eqn_rect (fun (γ₀ : forall q (α : q ≤ p), Γ q)
+              (e₀ : eqn (ext_typ_ctx (γ p !)) γ₀) =>
+        let e₁ := rew (fun γ₁ => forall (r : ℙ) (β : r ≤ q), ctx_rel Γ (β · (α · γ₁))) e₀ (α · (γ p !).(ext_typ_rel)) in
+        elt
+          (trm_elt P q (α · γ₀) e₁ 
+             (fun (r : ℙ) (β : r ≤ q) =>
+              eqn_rect
+                (fun (γ₀ : forall s : ℙ, s ≤ r -> Γ s)
+                     (_ : eqn (ext_typ_ctx (γ r (β ∘ α))) γ₀) => 
+                 Nat₀ r)
+                (ext_typ_ext (γ r (β ∘ α)))
+                (ext_rel_ctx (γε r (β ∘ α)) r !)
+              )
+             (fun (r : ℙ) (β : r ≤ q) => ext_rel_ext (γε r (β ∘ α)) r !)) q
+          !
+
+        ) _ (ext_rel_ctx (γε p !) p !)
+      ).
+    simpl.
+    pose (pO.(trm_elt) q (α · ext_typ_ctx (γ p !)) (α · ext_typ_rel (γ p !))).
+simpl in t.
+    refine 
+
+  - simpl.
+  fix F 1; intros n₀ e₀.
+  unshelve econstructor.
+  - refine (fun q α => _); simpl.
+    
+    refine (
+      match n₀ return eqn n₀ (ext_typ_ext (γ p !)) -> _
+      with
+      | O₀ _ => fun e => _
+      | S₀ _ n => fun e => _
+      end e₀
+    ).
+    * induction ((Nat_O_inv _ _ nε e)).
+      refine (pO.(trm_elt) _ _ _).
+    * induction (Nat_S_inv _ _ nε _ e).
+      unshelve refine (pS.(trm_elt) q (α · γ) (α · γε) n _ _ _).
+      
+2:{ simpl.
+  refine (fun q α => F
+    apply 
+
+refine (eqn_rect (fun n₀ => _) (Nat_O_inv _ _ _ e) _).
